iris/UkShRun.v
@@ -492,7 +492,7 @@ Section UkShRun.
     WP (Loop : expr riscv_lang).
   Proof.
     intros Hns He1 He2 Ha Hal Hrd. iIntros "#Hi Hw Hrun Hcont".
-    iDestruct "Hrun" as (xi C pt Rfd Rut sz M pm fdv cw gn cs pidv) "(%Hlo & %Hpm & %Hlzf & %HRut & Hheap & Hstk & Hufd & Hcwda & Hcha & #Hmy & #Hdep & Hb)".
+    iDestruct "Hrun" as (xi C pt Rfd Rut sz M pm fdv cw gn cs pidv) "(%Hlo & %Hpm & %Hlzf & %HRut & Hheap & Hstk & Hufd & Hcwda & Hcha & #Hmy & #Hdep & #Hnpx & Hb)".
     iDestruct (uinstr_is_uk_instr with "Hheap Hi") as %Hui.
     iDestruct (uheap_access (ukn_t N) (ukn_d N) (ukn_s N) M pm sz dq a 8 (nth_byte w)
                  ltac:(lia) ltac:(right; right; right; reflexivity) Hal
@@ -510,7 +510,7 @@ Section UkShRun.
               Hcan Hpg Hal8
               ltac:(rewrite Hua; exact Hmap)
               with "Hb [Hheap Hstk Hufd Hcwda Hcha Hw Hcont]").
-    iApply (urun_close_upd _ _ _ m rd _ _ _ _ _ _ _ _ _ Hns with "Hheap Hstk Hufd Hcwda Hcha Hmy Hdep").
+    iApply (urun_close_upd _ _ _ m rd _ _ _ _ _ _ _ _ _ Hns with "Hheap Hstk Hufd Hcwda Hcha Hmy Hdep Hnpx").
     iApply ("Hcont" with "Hw").
   Qed.
 
@@ -535,7 +535,7 @@ Section UkShRun.
     WP (Loop : expr riscv_lang).
   Proof.
     intros Hns He1 He2 Ha Hal Hrd. iIntros "#Hi Hw Hrun Hcont".
-    iDestruct "Hrun" as (xi C pt Rfd Rut sz M pm fdv cw gn cs pidv) "(%Hlo & %Hpm & %Hlzf & %HRut & Hheap & Hstk & Hufd & Hcwda & Hcha & #Hmy & #Hdep & Hb)".
+    iDestruct "Hrun" as (xi C pt Rfd Rut sz M pm fdv cw gn cs pidv) "(%Hlo & %Hpm & %Hlzf & %HRut & Hheap & Hstk & Hufd & Hcwda & Hcha & #Hmy & #Hdep & #Hnpx & Hb)".
     iDestruct (uinstr_is_uk_instr with "Hheap Hi") as %Hui.
     iDestruct (uheap_access (ukn_t N) (ukn_d N) (ukn_s N) M pm sz dq a 4 (nth_byte wv)
                  ltac:(lia) ltac:(right; right; left; reflexivity) Hal
@@ -553,7 +553,7 @@ Section UkShRun.
               Hcan Hpg Hal8
               ltac:(rewrite Hua; exact Hmap) eq_refl
               with "Hb [Hheap Hstk Hufd Hcwda Hcha Hw Hcont]").
-    iApply (urun_close_upd _ _ _ m rd _ _ _ _ _ _ _ _ _ Hns with "Hheap Hstk Hufd Hcwda Hcha Hmy Hdep").
+    iApply (urun_close_upd _ _ _ m rd _ _ _ _ _ _ _ _ _ Hns with "Hheap Hstk Hufd Hcwda Hcha Hmy Hdep Hnpx").
     iApply ("Hcont" with "Hw").
   Qed.
 
@@ -576,7 +576,7 @@ Section UkShRun.
     WP (Loop : expr riscv_lang).
   Proof.
     intros Hns Ha Hal Hrd. iIntros "#Hi Hw Hrun Hcont".
-    iDestruct "Hrun" as (xi C pt Rfd Rut sz M pm fdv cw gn cs pidv) "(%Hlo & %Hpm & %Hlzf & %HRut & Hheap & Hstk & Hufd & Hcwda & Hcha & #Hmy & #Hdep & Hb)".
+    iDestruct "Hrun" as (xi C pt Rfd Rut sz M pm fdv cw gn cs pidv) "(%Hlo & %Hpm & %Hlzf & %HRut & Hheap & Hstk & Hufd & Hcwda & Hcha & #Hmy & #Hdep & #Hnpx & Hb)".
     iDestruct (uinstr_is_uk_instr with "Hheap Hi") as %Hui.
     iDestruct (uheap_access (ukn_t N) (ukn_d N) (ukn_s N) M pm sz dq a 4 (nth_byte wv)
                  ltac:(lia) ltac:(right; right; left; reflexivity) Hal
@@ -591,7 +591,7 @@ Section UkShRun.
               Hcan Hpg Hal8
               ltac:(rewrite Hua; exact Hmap) eq_refl
               with "Hb [Hheap Hstk Hufd Hcwda Hcha Hw Hcont]").
-    iApply (urun_close_upd _ _ _ m rd _ _ _ _ _ _ _ _ _ Hns with "Hheap Hstk Hufd Hcwda Hcha Hmy Hdep").
+    iApply (urun_close_upd _ _ _ m rd _ _ _ _ _ _ _ _ _ Hns with "Hheap Hstk Hufd Hcwda Hcha Hmy Hdep Hnpx").
     iApply ("Hcont" with "Hw").
   Qed.
 
